Main.lean
@@ -3,6 +3,7 @@ import SSC.Contexts
 import SSC.Decompose
 import SSC.Reduction
 import SSC.Examples
+import SSC.Strategy
 import SSC.NormalForms
 import SSC.Theorems.WeakNormalImpliesNormal
 
